temp ghostptrtoken without refined

theories/typing/lib/ghostptrtoken/ghostptrtoken.v
@@ -1,11 +1,12 @@
 From lrust.typing Require Export type.
 From lrust.typing Require Import array_util typing.
+From lrust.typing.lib.ghostptrtoken Require Import permdata ghostseq.
 Set Default Proof Using "Type".
 
 Open Scope nat.
 Implicit Type 𝔄 𝔅: syn_type.
 
-Notation "'[∗' 'list]' ( k , x ) ∈ l , P" := ((big_opL bi_sep (fun _ '(k, x) => P) l))%core
+Notation "'[∗' 'list]' ( k , x ) ∈ l , P" := ((big_sepL (fun _ '(k, x) => P) l))%core
 (at level 200, l at level 10, k, x at level 1, right associativity)
   : bi_scope.
 
@@ -40,28 +41,67 @@ Section token.
 
   Definition alapply {A B K} (fl: list (K*(B → A))) (x: B) := (al_fmap (.$ x) fl).
 
-  Lemma split_mt_token {𝔄} d l' alπ Φ :
-    (l' ↦∗: (λ vl, [S(d') := d] ∃ (aπl: list (loc * (proph 𝔄))),
-      ⌜vl = [] ∧ alπ = alapply aπl⌝ ∗ Φ d' aπl)) ⊣⊢
-    [S(d') := d] ∃(aπl: list (loc * (proph 𝔄))),
-      ⌜alπ = alapply aπl⌝ ∗ l' ↦∗ [] ∗ Φ d' aπl.
-  Proof.
-    iSplit.
-    - iIntros "(%& ↦ & big)". case d=>// ?. iDestruct "big" as (?[->->]) "Φ".
-      iExists _. iSplit; [done|iFrame].
-    - iIntros "big". case d=>// ?. iDestruct "big" as (?->) "(↦ & ?)".
-      iExists []. iFrame "↦". iExists _. by iFrame.
+
+  Program Definition ghostptrtoken_ty {𝔄} (ty: type 𝔄) : type (listₛ (locₛ * 𝔄)) :=
+   (ghostseq_ty (permdata_ty ty)).
+  
+
+  Lemma ghostptrtoken_own_alt {𝔄} (ty: type 𝔄) alπ d tid vl:
+    ty_own (ghostptrtoken_ty ty) alπ d tid vl ⊣⊢
+      ∃(aπl: list (loc * (proph 𝔄))),
+        ⌜vl = [] ∧ alπ = alapply aπl⌝ ∗
+        ([∗ list] (l, aπ) ∈ aπl, [S(d') := d] ▷ l ↦∗: ty.(ty_own) aπ d' tid) ∗
+        ([∗ list] (l, aπ) ∈ aπl, freeable_sz' ty.(ty_size) l).
+  Proof. iSplit; iIntros "(%&(->&->)&X)"; iStopProof; 
+    (induction aπl; [iIntros "_"; iExists []; do 4 (iSplit||iModIntro||done)|]).
+    - iIntros "((%&%&(_&->)&X)&rest)". iDestruct (IHaπl with "rest") as "(%&(_&%)&tys&frees)". iExists ((l, vπ') :: aπl0).
+    iSplit. iPureIntro. split; [done|]. fun_ext=>π. simpl. by rewrite H.
+    destruct d; [done|]. iFrame. iDestruct "X" as "($&free)". rewrite freeable_sz_full. done.
+    - simpl. destruct a. iIntros "((ty&tys)&(free&frees))".
+    iDestruct (IHaπl with "[$tys $frees]") as "(%&(_&%)&X)". iExists (_ :: aπl0).
+    iSplit. iPureIntro. split; [done|]. fun_ext=>π. simpl. by rewrite H.
+    iFrame. iExists _, _. iSplit; [done|]. destruct d; iFrame. rewrite freeable_sz_full. done.
   Qed.
 
-  Lemma split_mt_token' {𝔄} l' alπ Φ :
-    (l' ↦∗: (λ vl, ∃(aπl: list (loc * (proph 𝔄))),
-      ⌜vl = [] ∧ alπ = alapply aπl⌝ ∗ Φ aπl)) ⊣⊢
+  Lemma ghostptrtoken_shr_alt {𝔄} (ty: type 𝔄) alπ d κ tid l:
+  ty_shr (ghostseq_ty (permdata_ty ty)) alπ d κ tid l ⊣⊢
     ∃(aπl: list (loc * (proph 𝔄))),
-      ⌜alπ = alapply aπl⌝ ∗ l' ↦∗ [] ∗ Φ aπl.
-  Proof.
-    set Φ' := λ _: nat, Φ. have ->: Φ = Φ' 0 by done.
-    by apply (split_mt_token (S _)).
+    ⌜alπ = alapply aπl⌝ ∗
+    ([∗ list] (l, aπ) ∈ aπl, [S(d') := d] ▷ ty.(ty_shr) aπ d' κ tid l).
+  Proof. iSplit; iIntros "(%&->&X)"; iStopProof; 
+    (induction aπl; [iIntros "_"; iExists []; do 4 (iSplit||iModIntro||done)|]).
+    - iIntros "((%&%&->&X)&rest)". iDestruct (IHaπl with "rest") as "(%&%&tys)". iExists ((l0, vπ') :: aπl0).
+    iSplit. iPureIntro. fun_ext=>π. simpl. by rewrite H.
+    destruct d; [done|]. iFrame.
+    - simpl. destruct a. iIntros "(ty&tys)".
+    iDestruct (IHaπl with "tys") as "(%&%&X)". iExists (_ :: aπl0).
+    iSplit. iPureIntro. fun_ext=>π. simpl. by rewrite H.
+    iFrame. iExists _, _. iSplit; [done|]. destruct d; iFrame.
   Qed.
+
+  Lemma split_mt_token {𝔄} (ty: type 𝔄) l' alπ d tid :
+  (l' ↦∗: ty_own (ghostptrtoken_ty ty) alπ d tid ) ⊣⊢
+  ∃(aπl: list (loc * (proph 𝔄))),
+    ⌜alπ = alapply aπl⌝ ∗ l' ↦∗ [] ∗         
+    ([∗ list] (l, aπ) ∈ aπl, [S(d') := d] ▷ l ↦∗: ty.(ty_own) aπ d' tid) ∗
+    ([∗ list] (l, aπ) ∈ aπl, freeable_sz' ty.(ty_size) l).
+  Proof. setoid_rewrite ghostptrtoken_own_alt.
+    iSplit. iIntros "(%&↦&%&(->&?)&ty)". iExists _. iFrame.
+    iIntros "(%&->&↦&ty)". iExists []. iFrame. iExists _. iFrame. done.
+  Qed.
+(* 
+Lemma split_mt_token {𝔄} d l' alπ Φ :
+  (l' ↦∗: (λ vl, [S(d') := d] ∃ (aπl: list (proph (loc * 𝔄))),
+    ⌜vl = [] ∧ alπ = lapply aπl⌝ ∗ Φ d' aπl)) ⊣⊢
+  [S(d') := d] ∃(aπl: list (loc * (proph 𝔄))),
+    ⌜alπ = alapply aπl⌝ ∗ l' ↦∗ [] ∗ Φ d' aπl.
+Proof.
+  iSplit.
+  - iIntros "(%& ↦ & big)". case d=>// ?. iDestruct "big" as (?[->->]) "Φ".
+    iExists _. iSplit; [done|iFrame].
+  - iIntros "big". case d=>// ?. iDestruct "big" as (?->) "(↦ & ?)".
+    iExists []. iFrame "↦". iExists _. by iFrame.
+Qed.
 
   Lemma ty_share_big_sepAL {𝔄} (ty: type 𝔄) E aπl d κ tid q :
     ↑lftN ⊆ E → lft_ctx -∗ κ ⊑ ty_lft ty -∗
@@ -97,7 +137,7 @@ Section token.
       iSplitL "↦ ty".
       { iExists _. iFrame. }
       iApply ("IH" with "↦s tys").
-  Qed.
+  Qed. *)
 
   (* Lemma remove_alapply {A B} `{Countable K} (aπl: gmap K (A → B)):
     alapply aπl = λ π, list_to_map (prod_map id (.$ π) <$> (map_to_list aπl)).
@@ -115,121 +155,6 @@ Section token.
     unfold prod_map. unfold uncurry. unfold Datatypes.uncurry. unfold fst. unfold snd. unfold id. reflexivity.
   Qed.
 
-  Lemma ty_own_proph_big_sepAL_mt {𝔄} (ty: type 𝔄) (n: nat) E aπl d tid κ q :
-  ↑lftN ⊆ E → lft_ctx -∗ κ ⊑ ty_lft ty -∗
-  ([∗ list] (l, aπ) ∈ aπl, l ↦∗: ty.(ty_own) aπ d tid) -∗ q.[κ]
-    ={E}=∗ |={E}▷=>^d |={E}=> ∃ξll q', ⌜Forall2 ty.(ty_proph) aπl.*2 ξll⌝ ∗ q':+[mjoin ξll] ∗
-      (q':+[mjoin ξll] ={E}=∗
-        ([∗ list] (l, aπ) ∈ aπl, l ↦∗: ty.(ty_own) aπ d tid) ∗ q.[κ]).
-  Proof.
-    rewrite {1} trans_big_sepAL_mt_ty_own. iIntros (?) "LFT In (%& ↦ & tys) κ".
-    iMod (ty_own_proph_big_sepL with "LFT In tys κ") as "Upd"; [done|].
-    iApply (step_fupdN_wand with "Upd"). iIntros "!> >(%&%&(%&->&%)& ξl & Totys) !>".
-    iExists _, _. rewrite vec_to_list_map vec_to_list_to_vec in H0.
-    iSplit; [done|]. iIntros "{$ξl}ξl".
-    iMod ("Totys" with "ξl") as "[tys $]".
-    rewrite trans_big_sepAL_mt_ty_own.
-    iModIntro. iExists _. iFrame.
-  Qed.
-
-  Lemma ty_shr_proph_big_sepAL {𝔄} (ty: type 𝔄) (n: nat) E aπl d κ tid κ' q :
-  ↑lftN ⊆ E → lft_ctx -∗ κ' ⊑ κ -∗ κ' ⊑ ty_lft ty -∗
-  ([∗ list] (l, aπ) ∈ aπl, ty.(ty_shr) aπ d κ tid l) -∗ q.[κ']
-    ={E}▷=∗ |={E}▷=>^d |={E}=> ∃ξll q', ⌜Forall2 ty.(ty_proph) aπl.*2 ξll⌝ ∗ q':+[mjoin ξll] ∗
-      (q':+[mjoin ξll] ={E}=∗ q.[κ']).
-  Proof.
-    iIntros (?) "#LFT #In #In' tys κ'".
-    unfold alapply.
-    iInduction aπl as [|[l x]] "IH" forall (q) =>/=.
-    { iApply step_fupdN_full_intro. iIntros "!>!>!>!>". iExists [], 1%Qp.
-      iFrame "κ'". iSplit. done. iSplit; [done|]. by iIntros. }
-    iDestruct "κ'" as "[κ' κ'₊]". iDestruct "tys" as "[ty tys]".
-    iMod (ty_shr_proph with "LFT In In' ty κ'") as "Upd"; [done|].
-    iMod ("IH" with "tys κ'₊") as "Upd'".
-    iIntros "!>!>". iCombine "Upd Upd'" as "Upd". iApply (step_fupdN_wand with "Upd").
-    iIntros "[>(%&%&%& ξl & Toκ') >(%&%&%& ζl & Toκ'₊)] !>".
-    iDestruct (proph_tok_combine with "ξl ζl") as (?) "[ξζl Toξζl]".
-    iExists _, _. iSplit. iPureIntro. by constructor. iFrame "ξζl". 
-    iIntros "ξζl". iDestruct ("Toξζl" with "ξζl") as "[ξl ζl]".
-    iMod ("Toκ'" with "ξl") as "$". by iMod ("Toκ'₊" with "ζl") as "$".
-  Qed.
-
-  Definition big_sepAL {K A} (Φ: K → A → iProp Σ) (l: list (K*A)) :=  ([∗ list] (k, x) ∈ l, Φ k x)%I.
-
-  (* Lemma all_share_peristent {𝔄} (ty: type 𝔄) aπl d' κ tid : Persistent (all_share 𝔄 ty aπl d' κ tid).
-  apply big_sepAL_persistent. intros. apply ty_shr_persistent. Qed. *)
-
-  (* Rust's GhostPtrToken<T> *)
-  Program Definition ghostptrtoken_ty {𝔄} (ty: type 𝔄) : type (listₛ (locₛ * 𝔄)) := {|
-    ty_size := 0;  ty_lfts := ty.(ty_lfts);  ty_E := ty.(ty_E);
-    ty_proph alπ ξl := exists (aπl: list (loc * (proph 𝔄))) ξll,
-      ξl = mjoin ξll /\ alπ = alapply aπl /\ Forall2 ty.(ty_proph) aπl.*2 ξll;
-    ty_own alπ d tid vl :=
-      [S(d') := d] ∃(aπl: list (loc * (proph 𝔄))),
-        ⌜vl = [] ∧ alπ = alapply aπl⌝ ∗
-        ▷ (big_sepAL (λ l aπ, l ↦∗: ty.(ty_own) aπ d' tid) aπl) ∗
-        (big_sepAL (λ l _, freeable_sz' ty.(ty_size) l) aπl);
-    ty_shr alπ d κ tid l' :=
-      [S(d') := d] ∃(aπl: list (loc * (proph 𝔄))),
-        ⌜alπ = alapply aπl⌝ ∗
-        ▷ (big_sepAL (λ l aπ, ty.(ty_shr) aπ d' κ tid l) aπl);
-  |}%I.
-  Next Obligation.
-    iIntros (???[]??) "token //". by iDestruct "token" as (?[-> _]) "?".
-  Qed.
-  Next Obligation. unfold big_sepAL.
-    move=> ??[|?][|?]*/=; try (by iIntros); [lia|]. do 12 f_equiv.
-    apply ty_own_depth_mono. lia.
-  Qed.
-  Next Obligation. unfold big_sepAL.
-    move=> ??[|?][|?]*/=; try (by iIntros); [lia|]. do 8 f_equiv.
-    apply ty_shr_depth_mono. lia.
-  Qed.
-  Next Obligation. unfold big_sepAL.
-    move=> ?????[|?]*; [by iIntros|]. iIntros "#? (%&?& All)".
-    iExists _. iSplit; [done|]. iNext.
-    erewrite !big_sepL_forall; [|intros ?[??]; by apply ty_shr_persistent ..]. iIntros (?[??]?).
-    iApply ty_shr_lft_mono; by [|iApply ("All" $! _ (_,_))].
-  Qed.
-  Next Obligation.
-    iIntros (???? d) "*% #LFT In Bor κ". rewrite split_mt_token. case d.
-    { by iMod (bor_persistent with "LFT Bor κ") as "[>[] _]". }
-    move=> ?. do 1 (iMod (bor_exists_tok with "LFT Bor κ") as (?) "[Bor κ]"; [done|]).
-    iMod (bor_sep_persistent with "LFT Bor κ") as "(>-> & Bor & κ)"; [done|].
-    iMod (bor_sep with "LFT Bor") as "[Bor↦ Bor]"; [done|].
-    iMod (bor_fracture (λ q', _ ↦∗{q'} _)%I with "LFT Bor↦") as "Bor↦"; [done|].
-    iMod (bor_sep with "LFT Bor") as "[Bor _]"; [done|].
-    iMod (bor_later_tok with "LFT Bor κ") as "Borκ"; [done|].
-    iIntros "/=!>!>!>". iMod "Borκ" as "[Bor κ]".
-    iMod (ty_share_big_sepAL with "LFT In Bor κ") as "Toshrs"; [done|].
-    iApply (step_fupdN_wand with "Toshrs"). iIntros "!> >[?$] !>".
-    iExists _. by iFrame.
-  Qed.
-  Next Obligation.
-    iIntros (????[|?]) "*% LFT In token κ/="; [done|].
-    iDestruct "token" as (?[->->]) "(↦tys & †)". iIntros "!>!>!>".
-    iMod (ty_own_proph_big_sepAL_mt with "LFT In ↦tys κ") as "Upd"; [done|done|].
-    iApply (step_fupdN_wand with "Upd"). iIntros "!> >(%&%&%& ξl & Totys) !>".
-    iExists _, _. iSplit. iExists _, _. done.
-    iIntros "{$ξl}ξl". iMod ("Totys" with "ξl") as "[tys $]". iModIntro.
-    iExists _. by iFrame.
-  Qed.
-  Next Obligation.
-    iIntros (????[|?]) "*%*% LFT In In' token κ'/="; [done|].
-    iDestruct "token" as (?->) "tys". iIntros "!>!>!>".
-    iMod (ty_shr_proph_big_sepAL with "LFT In In' tys κ'") as "Toκ'"; [done|done|].
-    iIntros "!>!>". iApply (step_fupdN_wand with "Toκ'").
-    iIntros ">(%&%&%& ξl & Toκ') !>". iExists _, _. iSplit. iExists _, _. done.
-    iIntros "{$ξl}ξl". by iMod ("Toκ'" with "ξl") as "$".
-  Qed.
-  Next Obligation.
-    simpl. intros ????(?&?&->&->&?). unfold alapply.
-    eassert (proph_dep _ _ _); [|unfold proph_dep; setoid_rewrite <- zip_to_prod_map; exact H0].
-    apply proph_dep_constr. by eapply ty_proph_weaken_big_sepL'.
-  Qed.
-
   Global Instance ghostptrtoken_ty_ne {𝔄} : NonExpansive (@ghostptrtoken_ty 𝔄).
-  Proof.
-    rewrite /ghostptrtoken_ty /big_sepAL. solve_ne_type; simpl. done.
-  Qed.
+  Proof. solve_ne_type. done. Qed.
 End token.
