theories/typing/lib/ghostptrtoken/ghostptrtoken_basic.v
@@ -1,6 +1,6 @@
 From lrust.typing Require Export type.
 From lrust.typing Require Import array_util typing.
-From lrust.typing.lib.ghostptrtoken Require Import ghostptrtoken.
+From lrust.typing.lib.ghostptrtoken Require Import ghostptrtoken ghostseq_basic permdata_basic.
 Set Default Proof Using "Type".
 
 Open Scope nat.
@@ -9,7 +9,7 @@ Implicit Type 𝔄 𝔅: syn_type.
 Section ghostptrtoken_basic.
   Context `{!typeG Σ}.
 
-  Lemma real_big_sepM_ty_shr {𝔄 𝔅} (ty: type 𝔄) (f: 𝔄 → 𝔅)
+  (* Lemma real_big_sepM_ty_shr {𝔄 𝔅} (ty: type 𝔄) (f: 𝔄 → 𝔅)
     aπl (d: nat) κ tid E L F q :
     real E L ty f → ↑lftN ⊆ F → lft_ctx -∗ elctx_interp E -∗ llctx_interp L q -∗
     ([∗ list] (l, aπ) ∈ aπl, ty.(ty_shr) aπ d κ tid l)
@@ -25,39 +25,20 @@ Section ghostptrtoken_basic.
     iApply (step_fupdN_wand with "Upd"). iIntros "[>(%Eq &$&$) >(%Eq' &$&$)] !%".
     move: Eq=> [b Eq]. move: Eq'=> [bm Eq']. exists ((l,b) :: bm).
     fun_ext=>/= π. by move: (equal_f Eq π) (equal_f Eq' π)=>/= <-<-.
-  Qed.
+  Qed. *)
 
   Global Instance token_type_contractive 𝔄 : TypeContractive (ghostptrtoken_ty (𝔄:=𝔄)).
-  Proof.
-    rewrite /ghostptrtoken_ty /big_sepAL.
-    split; [done|split| |]; simpl.
-    - by apply type_lft_morphism_id_like.
-    - intros. do 6 f_equiv. intros ?. by eapply Forall2_impl.
-    - intros ???(?&?&->&->&?). eexists _, _. split. exact H. 
-      intros. eexists _, _. done.  
-    - move=>/= > ->*. do 14 (f_contractive || f_equiv). by simpl in *.
-    - intros ??????????????. unfold ty_shr. unfold ghostptrtoken_ty. do 10 (f_contractive || f_equiv). by simpl in *.
-  Qed.
+  Proof. solve_typing. Qed.
 
   Global Instance token_send {𝔄} (ty: type 𝔄) : Send ty → Send (ghostptrtoken_ty ty).
-  Proof. rewrite /ghostptrtoken_ty /big_sepAL. move=> ?>/=. by do 14 (f_equiv || move=>?). Qed.
+  Proof. solve_typing. Qed.
 
   Global Instance token_sync {𝔄} (ty: type 𝔄) : Sync ty → Sync (ghostptrtoken_ty ty).
-  Proof. rewrite /ghostptrtoken_ty /big_sepAL. move=> ?>/=. by do 10 (f_equiv || move=>?). Qed.
+  Proof. solve_typing. Qed.
 
   Lemma token_resolve {𝔄} (ty: type 𝔄) Φ E L :
-    resolve E L ty Φ → resolve E L (ghostptrtoken_ty ty) ((lforall Φ) ∘ (fmap snd)).
-  Proof.
-    iIntros (????[|]???) "#LFT #PROPH #E L token //=".
-    unfold big_sepAL.
-    iDestruct "token" as (?[->->]) "[↦tys _]". iIntros "!>!>!>".
-    rewrite trans_big_sepAL_mt_ty_own. iDestruct "↦tys" as (?) "[↦ tys]".
-    iMod (resolve_big_sepL_ty_own with "LFT PROPH E L tys") as "Upd"; [done..|].
-    iApply (step_fupdN_wand with "Upd").
-    rewrite vec_to_list_map. rewrite vec_to_list_to_vec.
-    unfold lapply. setoid_rewrite <- list_fmap_compose. setoid_rewrite lforall_Forall.
-    setoid_rewrite Forall_fmap. by iIntros "!> H".
-  Qed.
+    resolve E L ty Φ → resolve E L (ghostptrtoken_ty ty) (lforall (Φ ∘ snd)).
+  Proof. intros. by apply permdata_resolve, seq_resolve in H. Qed.
 
   Lemma token_resolve_just {𝔄} (ty: type 𝔄) E L :
     resolve E L ty (const True) → resolve E L (ghostptrtoken_ty ty) (const True).
@@ -65,49 +46,14 @@ Section ghostptrtoken_basic.
 
   Lemma token_real {𝔄 𝔅} (ty: type 𝔄) (f: 𝔄 → 𝔅) E L :
     real E L ty f → real (𝔅:=listₛ (locₛ*_) ) E L (ghostptrtoken_ty ty) (al_fmap f).
-  Proof.
-    move=> Rl. split; iIntros (???[|]) "*% LFT E L token //="; unfold big_sepAL.
-    - iDestruct "token" as (?[->->]) "[↦tys †]". iIntros "!>!>!>".
-      rewrite trans_big_sepAL_mt_ty_own. iDestruct "↦tys" as (?) "[↦ tys]".
-      iMod (real_big_sepL_ty_own with "LFT E L tys") as "Upd"; [done..|].
-      iApply (step_fupdN_wand with "Upd"). iIntros "!> >(%Eq &$&?) !>".
-      iSplit; last first.
-      { iExists _. iFrame "†". iSplit; [done|]. iNext.
-        rewrite trans_big_sepAL_mt_ty_own. iExists _. iFrame. }
-      iPureIntro. move: Eq=> [bl Eq]. exists (zip aπl.*1 (vec_to_list bl)). fun_ext=>/= π.
-      move: (equal_f Eq π)=>/= <-.
-      rewrite 3! vec_to_list_map  vec_to_list_to_vec.
-      rewrite -list_fmap_compose zip_to_prod_map /alapply -list_fmap_compose.
-      reflexivity.
-    - iDestruct "token" as (?) "[%Bor tys]". iIntros "!>!>!>".
-      iMod (real_big_sepM_ty_shr with "LFT E L tys") as "Upd"; [done..|].
-      iIntros "!>!>". iApply (step_fupdN_wand with "Upd").
-      iIntros ">(%Eq &$& tys) !>". iSplit; [|iExists _; by iFrame].
-      iPureIntro. move: Eq=> [bl Eq]. exists bl. fun_ext=>/= π.
-      move: (equal_f Eq π)=>/= <-.  by rewrite Bor.
-  Qed.
+  Proof. intros. by apply permdata_real, seq_real in H. Qed.
 
   Lemma token_subtype {𝔄 𝔅} (f: 𝔄 → 𝔅) ty ty' E L :
     subtype E L ty ty' f → subtype E L (ghostptrtoken_ty ty) (ghostptrtoken_ty ty') (al_fmap f).
-  Proof.
-    iIntros (Sub ?) "L". iDestruct (Sub with "L") as "#Sub". iIntros "!> E".
-    iDestruct ("Sub" with "E") as "((%EqSz&%Proph) &?&#Own&#Shr)".
-    have Eq: ∀(aπl: list (loc*(proph 𝔄))), al_fmap f ∘ alapply aπl = alapply (al_fmap (f ∘.) aπl).
-    { move=> ?. fun_ext=>/= ?. f_equal. unfold alapply. rewrite -2! list_fmap_compose. reflexivity. }
-    iSplit. iPureIntro. split; [done|]. intros ??(?&?&->&->&?).
-    rewrite Eq. eexists _, _. do 2 (split; [done|]). rewrite 2! Forall2_fmap_l. rewrite Forall2_fmap_l in H.
-    eapply Forall2_impl. done. simpl. intros. by apply Proph.
-    iSplit; [done|]. iSplit; iIntros "!>" (?[|]) "* token //="; unfold big_sepAL.
-    - iDestruct "token" as (?[->->]) "(↦tys & †)". iExists  _.
-      iSplit; [done|]. rewrite 2! big_opL_fmap EqSz. simpl.
-      iSplitR "†"; [iNext|]; iApply (big_sepL_impl with "[$]");
-      iModIntro; iIntros (?[??]?). simpl. iIntros "(%vl&↦&tys)".
-      iExists _. iFrame. iApply "Own". done. simpl. iIntros. done.
-    - iDestruct "token" as (?->) "↦". iExists _. rewrite Eq.
-      iSplit; [done|].
-      rewrite big_opL_fmap. iApply (big_sepL_impl with "↦").
-      do 2 iModIntro. iIntros (???) "↦". destruct x. simpl. iApply ("Shr" with "↦").
+  Proof. 
+    intros. apply permdata_subtype, seq_subtype in H. done.
   Qed.
+
   Lemma token_eqtype {𝔄 𝔅} (f: 𝔄 → 𝔅) g ty ty' E L :
     eqtype E L ty ty' f g → eqtype E L (ghostptrtoken_ty ty) (ghostptrtoken_ty ty') (al_fmap f) (al_fmap g).
   Proof. move=> [??]. split; by apply token_subtype. Qed.
@@ -116,25 +62,20 @@ Section ghostptrtoken_basic.
   Definition ghostptrtoken_new: val :=
     fn: [] :=
       let: "r" := new [ #0] in
-      let: "dummy" := new [ #0] in
       return: ["r"].
 
   Lemma ghostptrtoken_new_type {𝔄} (ty: type 𝔄) :
     typed_val ghostptrtoken_new (fn(∅) → ghostptrtoken_ty ty) (λ post _, post []).
-  Proof.
+  Proof. Opaque ghostptrtoken_ty.
     eapply type_fn; [apply _|]=> _ ???. simpl_subst.
     iIntros (???) "_ #TIME _ _ _ Na L C _ Obs". iMod persistent_time_receipt_0 as "⧖".
     wp_bind (new _). iApply (wp_persistent_time_receipt with "TIME ⧖"); [done|].
     iApply wp_new; [done..|]. iIntros "!>" (l) "[† _] ⧖". wp_seq.
-    wp_bind (new _). iApply (wp_persistent_time_receipt with "TIME ⧖"); [done|].
-    iApply wp_new; [done..|]. iIntros "!>" (l') "[†' _] ⧖".
-    do 3 wp_seq.
+    do 2 wp_seq.
     rewrite cctx_interp_singleton.
     iApply ("C" $! [# #_] -[const []] with "Na L [-Obs] Obs"). iSplit; [|done].
-    iExists _, _. do 2 (iSplit; [done|]). rewrite/= freeable_sz_full split_mt_token'. 
-    iFrame "†". iNext. iExists []. iSplit.
-    iPureIntro. apply functional_extensionality. intros. unfold alapply. done.
-    unfold big_sepAL.
+    iExists _, _. do 2 (iSplit; [done|]). rewrite/= freeable_sz_full split_mt_token. 
+    iFrame "†". iNext. iExists []. iSplit. done.
     rewrite heap_mapsto_vec_nil 2! big_sepL_nil.
     iSplit; [done|done].
   Qed.
