theories/typing/lib/ghostptrtoken/ghostptrtoken_insertremove.v
@@ -16,9 +16,9 @@ Section ghostptrtoken_insertremove.
 
   (* Rust's GhostPtrToken::insert *)
   Lemma ghostptrtoken_insert_type {𝔄} (ty: type 𝔄) :
-    typed_val (ghostptrtoken_insert ty) (fn<α>(∅; &uniq{α} (ghostptrtoken_ty ty), box ty) → ptr)
-      (λ post '-[(al, al'); a], forall ptr, al' = (ptr,a)::al → ((ty.(ty_size) > 0) → NoDup al'.*1) → post ptr).
-  Proof.
+   (ty.(ty_size) > 0) → typed_val (ghostptrtoken_insert ty) (fn<α>(∅; &uniq{α} (ghostptrtoken_ty ty), box ty) → ptr)
+      (λ post '-[(al, al'); a], forall ptr, (list_to_gmap al') = <[ptr:=a]>(list_to_gmap al) → (list_to_gmap al) !! ptr = None → post ptr).
+  Proof. intros.
     eapply type_fn; [apply _|]=> α ??[l[x[]]]. simpl_subst.
     iIntros (?(lπ & bπ &[]) ?) "#LFT #TIME #PROPH #UNIQ #E Na L C /=(l & x &_) #Obs".
     rewrite !tctx_hasty_val. iDestruct "l" as ([|dl]) "[_ l]"=>//.
@@ -37,21 +37,22 @@ Section ghostptrtoken_insertremove.
     iMod (lctx_lft_alive_tok α with "E L") as (?) "(α & L & ToL)"; [solve_typing..|].
     iMod (bor_acc with "LFT Bor α") as "[(%&%& ⧖u & Pc & ↦token) ToBor]"; [done|].
     wp_seq. iDestruct (uniq_agree with "Vo Pc") as %[<-<-].
-    rewrite split_mt_token. case du as [|du]=>//=.
+    rewrite split_mt_token.
     iDestruct "↦token" as (aπl Eq1) "(↦l & ↦tys & †)".
     iCombine "⧖u ⧖x" as "#⧖". simpl.
     iMod (uniq_update with "UNIQ Vo Pc") as "[Vo Pc]"; [done|].
-    iAssert ((l' ↦∗: (ghostptrtoken_ty ty).(ty_own) _ (S (du `max` dx)) tid))%I with "[↦l ↦tys x' † †x']" as "own".
-    iExists _. iFrame. iExists ((p, bπ)::aπl). iSplit; [done|].
-    rewrite freeable_sz_full. iFrame. iNext.
-    unfold big_sepAL. rewrite big_sepL_cons. iSplitL "x'".
-    iDestruct "x'" as (?) "(↦&own)". iExists (vl). iFrame. iApply (ty_own_depth_mono with "own"). lia.
-    iApply (big_sepL_impl with "↦tys"). iModIntro. iIntros (?[??]?) "H".
-    iDestruct "H" as (?) "(H1&H2)". iExists vl. iFrame. iApply (ty_own_depth_mono with "H2"). lia.
-    iDestruct ((plain_entails_r (ghost_ptr_token_no_dup _ _ _ _ _)) with "own") as "(own&>%no_dup)".
+    iDestruct ((plain_entails_r (ghost_ptr_token_no_dup' _ ((p, bπ)::aπl) (du `max` (S dx)) _ H)) with "[↦tys x']") as "(↦tys&>%no_dup)".
+    { replace (du `max` (S dx)) with (S ((pred du) `max` dx)); [|lia]. simpl. 
+    iSplitL "x'". iNext. iApply (ty_own_mt_depth_mono with "x'"); lia.
+    iApply (big_sepL_impl with "↦tys"). iModIntro. iIntros (?[??]?) "H". destruct du; [done|].
+    iApply (ty_own_mt_depth_mono with "H"); lia. }
+    iAssert ((l' ↦∗: (ghostptrtoken_ty ty).(ty_own) _ _ tid))%I with "[↦l ↦tys † †x']" as "own".
+    iApply split_mt_token. iExists ((p, bπ)::aπl). 
+    rewrite freeable_sz_full. iFrame. done.
     iMod ("ToBor" with "[own Pc]") as "[Bor α]".
     iDestruct (bi.later_intro with "own") as "own". 
-    iNext. iExists _, _. iFrame "⧖ Pc own".
+    iNext. iExists _, _. setoid_rewrite split_mt_token. iFrame "⧖ Pc".
+    iClear "#". iStopProof. do 11 f_equiv.
     iMod ("ToL" with "α L") as "L".
     set lπ' := λ π, ((alapply ((p, bπ)::aπl) π), π ξ).
     iApply (type_type +[#l' ◁ &uniq{α} (ghostptrtoken_ty ty); #x ◁ box ptr] -[lπ'; const p]
@@ -67,7 +68,7 @@ Section ghostptrtoken_insertremove.
     - iApply proph_obs_impl; [|done]=> π.
       move: (equal_f Eq1 π) (equal_f Eq2 π)=>/=. case (lπ π)=>/= ??->-> Imp Eq.
       apply Imp. rewrite Eq. reflexivity.
-      intros. rewrite Eq. apply no_dup. done.
+      apply not_elem_of_list_to_map_1. rewrite -list_fmap_compose.  inversion_clear no_dup. done.
   Qed.
 
   Definition ghostptrtoken_remove {𝔄} (ty: type 𝔄) : val :=
@@ -75,10 +76,10 @@ Section ghostptrtoken_insertremove.
       delete [ #1; "t"];;
       return: ["ptr"].
 
-  (* Rust's GhostPtrToken::re,ove *)
+  (* Rust's GhostPtrToken::remove *)
   Lemma ghostptrtoken_remove_type {𝔄} (ty: type 𝔄) :
     typed_val (ghostptrtoken_remove ty) (fn<α>(∅; &uniq{α} (ghostptrtoken_ty ty), ptr) → box ty)
-      (λ post '-[(al, al'); p], exists(a: 𝔄), ((list_to_gmap al) !! p = Some a) ∧ ((<[p:=a]>(list_to_gmap al') = (list_to_gmap al)) → ((ty.(ty_size) > 0) → NoDup al.*1) → post a)).
+      (λ post '-[(al, al'); p], exists(a: 𝔄), ((list_to_gmap al) !! p = Some a) ∧ ((<[p:=a]>(list_to_gmap al') = (list_to_gmap al)) → post a)).
   Proof.
     eapply type_fn; [apply _|]=> α ??[l[x[]]]. simpl_subst.
     iIntros (?(lπ & pπ &[]) ?) "#LFT #TIME #PROPH #UNIQ #E Na L C /=(l & x &_) #Obs".
@@ -97,9 +98,8 @@ Section ghostptrtoken_insertremove.
     iMod (lctx_lft_alive_tok α with "E L") as (?) "(α & L & ToL)"; [solve_typing..|].
     iMod (bor_acc with "LFT Bor α") as "[(%&%& ⧖u & Pc & ↦token) ToBor]"; [done|].
     wp_seq. 
-    iDestruct ((plain_entails_r (ghost_ptr_token_no_dup _ _ _ _ _)) with "↦token") as "(↦token&>%no_dup)".
     iDestruct (uniq_agree with "Vo Pc") as %[<-<-].
-    rewrite split_mt_token. case du as [|du]=>//=.
+    rewrite split_mt_token.
     iDestruct "↦token" as (aπl Eq1) "(↦l & ↦token)".
     iCombine "⧖u ⧖x" as "#⧖". simpl.
     iMod (proph_obs_sat with "PROPH Obs") as "%ObsSat"; [done|].
@@ -109,16 +109,16 @@ Section ghostptrtoken_insertremove.
     destruct H1 as (?&Contains&?).
     rewrite /alapply list_to_map_fmap lookup_fmap Heqbπ in Contains. done.
     destruct (elem_of_list_to_map_2' _ _ _ Heqbπ) as (rπ&perm&reinsert).
-    unfold big_sepAL.
     iEval (rewrite perm 2! big_sepL_cons) in "↦token".
     iDestruct "↦token" as "((↦x' & ↦) & †x' & †)".
+    destruct du; [done|].
     iMod (uniq_update with "UNIQ Vo Pc") as "[Vo Pc]"; [done|].
-    assert ((S du `max` dx) = S(du `max` (pred dx))); [by lia|]. rewrite H1 /=.
+    replace (S du `max` dx) with (S (du `max` (pred dx))); [|lia].
     iMod ("ToBor" with "[↦l ↦ † Pc]") as "[Bor α]".
     { iNext. iExists _, _. rewrite split_mt_token. iFrame "⧖ Pc".
       iExists _. iFrame. iSplit; [done|].
-      iNext. iApply (big_sepL_impl with "↦"). iModIntro. iIntros (?[??]?) "H".
-      iDestruct "H" as (?) "(H1&H2)". iExists _. iFrame. iApply (ty_own_depth_mono with "H2"). fold max. lia.
+      iApply (big_sepL_impl with "↦"). iModIntro. iIntros (?[??]?) "H".
+      iDestruct "H" as (?) "(H1&H2)". iExists _. iFrame. iApply (ty_own_depth_mono with "H2"). lia.
     }
     iMod ("ToL" with "α L") as "L".
     set lπ' := λ π, ((alapply rπ π), π ξ).
@@ -144,8 +144,7 @@ Section ghostptrtoken_insertremove.
       rewrite lookup_eq in Heqbπ. injection Heqbπ as ->.
       apply Imp. rewrite Eq.
       rewrite /alapply 2! list_to_map_fmap -fmap_insert. f_equal.
-      rewrite (equal_f pπeq). exact. 
-      intros. rewrite -Eq1. apply no_dup. done.
+      rewrite (equal_f pπeq). exact.
   Qed.
     
 End ghostptrtoken_insertremove.
