theories/typing/lib/ghostptrtoken/heap_util.v
@@ -47,26 +47,20 @@ From lrust.typing Require Import ghostptrtoken.ghostptrtoken.
 Section defs2.
 Context `{!typeG Σ}.
 
-Lemma ghost_ptr_token_no_dup {𝔄} (ty: type 𝔄) l alπ d tid:
-    (l ↦∗: (ghostptrtoken_ty ty).(ty_own) alπ d tid) -∗ ▷⌜(ty.(ty_size) > 0) → forall π, NoDup (alπ π).*1⌝.
+Lemma ghost_ptr_token_no_dup {𝔄} (ty: type 𝔄) aπl d tid:
+    ([∗ list](l0, aπ)∈ aπl, [S(d') := d] ▷ (∃ vl : list val, l0 ↦∗ vl ∗ ty_own ty aπ d' tid vl)) -∗ ▷⌜(ty.(ty_size) > 0) → NoDup aπl.*1⌝.
 Proof.
-    iIntros "(%vl&_&↦l)". destruct d. done.
-    iDestruct "↦l" as "(%aπl&(->&->)&(↦l&_))".
-    iNext. unfold big_sepAL.
-    iIntros (? π).
-    iInduction aπl as [|[??]] "IH". rewrite NoDup_nil.  done.
-    rewrite /alapply fmap_cons fmap_cons NoDup_cons. simpl. iSplit.
-    iIntros (?).
-    iDestruct "↦l" as "(↦1&↦l)".
-    do 2 (rewrite elem_of_list_fmap in H; destruct H as ([??]&->&H)). simpl.
-    iDestruct (big_sepL_elem_of _ _ _ H with "↦l") as "↦2".
+    iInduction aπl as [|[??]] "IH". rewrite NoDup_nil. iIntros. done.
+    simpl. iIntros "(↦1&↦l)". rewrite NoDup_cons.
+    destruct d; [done|]. iIntros "%". iSplit.
+    iIntros (?). rewrite elem_of_list_fmap in H; destruct H as ([??]&->&H); simpl.
+    iDestruct (big_sepL_elem_of _ _ _ H with "↦l") as "↦2". iNext.
     iApply (no_duplicate_heap_mapsto_own with "↦1 ↦2"). lia.
-    iDestruct "↦l" as "(↦1&↦l)".
-    iApply "IH". iFrame.
+    iDestruct ("IH" with "↦l") as ">%". apply H in a. done. 
 Qed.
 
-Lemma ghost_ptr_token_no_dup' {𝔄} (ty: type 𝔄) l alπ d tid:
-    (ty.(ty_size) > 0) → (l ↦∗: (ghostptrtoken_ty ty).(ty_own) alπ d tid) -∗ ▷⌜forall π, NoDup (alπ π).*1⌝. 
+Lemma ghost_ptr_token_no_dup' {𝔄} (ty: type 𝔄) aπl d tid:
+  (ty.(ty_size) > 0) → ([∗ list](l0, aπ)∈ aπl, [S(d') := d] ▷ (∃ vl : list val, l0 ↦∗ vl ∗ ty_own ty aπ d' tid vl)) -∗ ▷⌜NoDup aπl.*1⌝.
 Proof.
     iIntros. iDestruct (ghost_ptr_token_no_dup with "[$]") as ">%X".
     specialize (X H). done.
