theories/typing/lib/ghostptrtoken/permdata_basic.v
@@ -1,0 +1,87 @@
+From lrust.typing Require Export type.
+From lrust.typing Require Import typing zst.
+From lrust.typing.lib.ghostptrtoken Require Import permdata.
+Set Default Proof Using "Type".
+
+Open Scope nat.
+Implicit Type 𝔄 𝔅: syn_type.
+
+Section permdata_basic.
+  Context `{!typeG Σ}.
+
+  Global Instance permdata_type_ne 𝔄 : TypeContractive (permdata_ty (𝔄:=𝔄)).
+  Proof.
+    split; [done|split| |]; simpl.
+    - by apply type_lft_morphism_id_like.
+    - intros. do 5 f_equiv. done.
+    - intros ???(?&?&->&?). eexists [_], [_]. split. by constructor. 
+      intros. eexists _, _. inversion_clear H0. done.  
+    - intros ???->**. do 12 (f_contractive || f_equiv). by simpl in *.
+    - intros **. do 8 (f_contractive || f_equiv). by simpl in *.
+  Qed.
+
+  Global Instance permdata_send {𝔄} (ty: type 𝔄) : Send ty → Send (permdata_ty ty).
+  Proof. move=> ?>/=. by do 12 (f_equiv || move=>?). Qed.
+
+  Global Instance permdata_sync {𝔄} (ty: type 𝔄) : Sync ty → Sync (permdata_ty ty).
+  Proof. move=> ?>/=. by do 8 (f_equiv || move=>?). Qed.
+
+  Lemma permdata_resolve {𝔄} (ty: type 𝔄) Φ E L :
+    resolve E L ty Φ → resolve E L (permdata_ty ty) (Φ ∘ snd).
+  Proof.
+    iIntros (????????) "#LFT #PROPH #E L token".
+    iDestruct "token" as (??[->->]) "box".
+    eapply own_resolve in H. by iApply (H with "LFT PROPH E L box").
+  Qed.
+
+  Lemma permdata_resolve_just {𝔄} (ty: type 𝔄) E L :
+    resolve E L ty (const True) → resolve E L (permdata_ty ty) (const True).
+  Proof. move=> ?. apply resolve_just. Qed.
+
+  Lemma permdata_real {𝔄 𝔅} (ty: type 𝔄) (f: 𝔄 → 𝔅) E L :
+    real E L ty f → real (𝔅:=locₛ * _) E L (permdata_ty ty) (prod_map id f).
+  Proof.
+    move=> Rl. split; iIntros (????) "*% LFT E L token".
+    - eapply own_real in Rl. destruct Rl as [Rlo _].
+      iDestruct "token" as (??[->->]) "own".
+      iMod (Rlo with "LFT E L own") as "Upd"; [done..|].
+      iApply (step_fupdN_wand with "Upd"). iIntros "!> >((%&%Eq) &$&?) !>".
+      iSplit; [|iExists _, _; by iSplit].
+      iPureIntro. exists (l, v). fun_ext=>/= π. simpl.
+      move: (equal_f Eq π)=>/= ->. done.
+    - destruct Rl as [_ Rls].
+      iDestruct "token" as (??) "(->&shr)". destruct d; [done|]. simpl.
+      iIntros "!>!>!>". iMod (Rls with "LFT E L shr") as "Upd"; [done..|].
+      iIntros "!>!>". iApply (step_fupdN_wand with "Upd").
+      iIntros ">((%&%Eq) &$& tys) !>". iSplit; [|iExists _, _; by iFrame].
+      iPureIntro. exists (l0, v). fun_ext=>/= π.
+      move: (equal_f Eq π)=>/= ->. done.
+  Qed.
+
+  Lemma permdata_subtype {𝔄 𝔅} (f: 𝔄 → 𝔅) ty ty' E L :
+    subtype E L ty ty' f → subtype E L (permdata_ty ty) (permdata_ty ty') (prod_map id f).
+  Proof.
+    iIntros (Sub ?) "L". iDestruct (Sub with "L") as "#Sub".
+    eapply box_subtype in Sub. iDestruct (Sub with "L") as "#SubO". iIntros "!> #E".
+    iDestruct ("Sub" with "E") as "((%EqSz&%Proph) &?&_&#Shr)".
+    iDestruct ("SubO" with "E") as "(_&_&#Own&_)".
+    have Eq: ∀ (l: loc) (vπ: (proph 𝔄)), (prod_map id f) ∘ (λ π, (l, vπ π)) = (λ π, (l, (f ∘ vπ) π)).
+    { move=> ??. fun_ext=>/= ?. done. }
+    iSplit. iPureIntro. split; [done|]. intros ??(?&?&->&?).
+    rewrite Eq. apply Proph in H. eexists _, _. done.
+    iSplit; [done|]. iSplit; iIntros "!>" (??) "* token".
+    - iDestruct "token" as (??[->->]) "tys". iExists  _, _.
+      iSplit; [done|]. by iApply "Own".
+    - iDestruct "token" as (??->) "token". destruct d; [done|]. iExists _, _.
+      rewrite Eq. iSplit; [done|]. iNext. by iApply "Shr".
+  Qed.
+  Lemma permdata_eqtype {𝔄 𝔅} (f: 𝔄 → 𝔅) g ty ty' E L :
+    eqtype E L ty ty' f g → eqtype E L (permdata_ty ty) (permdata_ty ty') (prod_map id f) (prod_map id g).
+  Proof. move=> [??]. split; by apply permdata_subtype. Qed.
+
+  Global Instance permdata_zst {𝔄} (ty: type 𝔄) : ZST (permdata_ty ty).
+  Proof. done. Qed.
+End permdata_basic.
+
+Global Hint Resolve permdata_resolve | 5 : lrust_typing.
+Global Hint Resolve permdata_resolve_just permdata_subtype permdata_eqtype : lrust_typing.
